\documentclass{article}
\usepackage{enumerate}
\usepackage{amsmath}
\usepackage{amssymb}
\usepackage{graphicx}
\usepackage{subfigure}
\usepackage{geometry}
\usepackage{caption}
\usepackage{indentfirst}
\geometry{left=3.0cm,right=3.0cm,top=3.0cm,bottom=4.0cm}
\usepackage{ctex}
\renewcommand{\thesection}{Ex.}
\title{MA318\ 偏微分方程\ 作业一}
\author{刘逸灏 515370910207}
\date{\today}

\begin{document}
\maketitle

\section{1.1/6}
$$\xi=x-at$$
$$\frac{\partial F(\xi)}{\partial x}=\frac{dF}{d\xi}\frac{\partial\xi}{\partial x}=F'(\xi)$$
$$\frac{\partial^2 F(\xi)}{\partial x^2}=\frac{\partial F'(\xi)}{\partial x}=\frac{dF'(\xi)}{d\xi}\frac{\partial\xi}{\partial x}=F''(\xi)$$
$$\frac{\partial F(\xi)}{\partial t}=\frac{dF}{d\xi}\frac{\partial\xi}{\partial t}=-aF'(\xi)$$
$$\frac{\partial^2 F(\xi)}{\partial t^2}=-a\frac{\partial F'(\xi)}{\partial t}=-a\frac{dF'(\xi)}{d\xi}\frac{\partial\xi}{\partial t}=a^2F''(\xi)$$
$$\frac{\partial^2 F(\xi)}{\partial t^2}-a^2\frac{\partial^2 F(\xi)}{\partial x^2}=0$$

同理，
$$\xi=x+at$$
$$\frac{\partial^2 G(\xi)}{\partial t^2}-a^2\frac{\partial^2 G(\xi)}{\partial x^2}=0$$

\section{1.1/7}
$$\frac{\partial u}{\partial t}=-t(t^2-x^2-y^2)^{-\frac{3}{2}}$$
$$\frac{\partial^2 u}{\partial t^2}=3t^2(t^2-x^2-y^2)^{-\frac{5}{2}}-(t^2-x^2-y^2)^{-\frac{3}{2}}=(t^2-x^2-y^2)^{-\frac{5}{2}}(3t^2-t^2+x^2+y^2)$$
$$\frac{\partial u}{\partial x}=x(t^2-x^2-y^2)^{-\frac{3}{2}}$$
$$\frac{\partial^2 u}{\partial x^2}=3x^2(t^2-x^2-y^2)^{-\frac{5}{2}}+(t^2-x^2-y^2)^{-\frac{3}{2}}=(t^2-x^2-y^2)^{-\frac{5}{2}}(3x^2+t^2-x^2-y^2)$$
$$\frac{\partial u}{\partial y}=y(t^2-x^2-y^2)^{-\frac{3}{2}}$$
$$\frac{\partial^2 u}{\partial y^2}=3y^2(t^2-x^2-y^2)^{-\frac{5}{2}}+(t^2-x^2-y^2)^{-\frac{3}{2}}=(t^2-x^2-y^2)^{-\frac{5}{2}}(3y^2+t^2-x^2-y^2)$$
$$3t^2-t^2+x^2+y^2=(3x^2+t^2-x^2-y^2)+(3y^2+t^2-x^2-y^2)$$
$$\frac{\partial^2 u}{\partial t^2}=\frac{\partial^2 u}{\partial x^2}+\frac{\partial^2 u}{\partial y^2}$$

\section{2.1/1}

\section{2.1/2}

\section{2.1/3}

\end{document}
 
